Add comments to first chapter

LeroyCompilerVerificationCourse/Imp.lean
@@ -6,15 +6,24 @@ Authors: Wojciech Różowski
 
 import LeroyCompilerVerificationCourse.Sequences
 
+/-
+  1. The source language: IMP
+    1.1 Arithmetic expressions
+-/
 def ident := String deriving BEq, Repr, Hashable
 
+-- The abstract syntax: an arithmetic expression is either...
 inductive aexp : Type where
-  | CONST (n : Int)
-  | VAR (x : ident)
-  | PLUS (a1 : aexp) (a2 : aexp)
-  | MINUS (a1 : aexp) (s2 : aexp)
+  | CONST (n : Int)               -- a constant, or
+  | VAR (x : ident)               -- a variable, or
+  | PLUS (a1 : aexp) (a2 : aexp)  -- a sum of two expressions, or
+  | MINUS (a1 : aexp) (s2 : aexp) -- a difference of two expressions
 
+/-
+The denotational semantics: an evaluation function that computes the integer value denoted by an expression.  It is parameterized by a store [s] that associates values to variables.
+-/
 def store : Type := ident → Int
+
 
 @[grind] def aeval (s : store) (a : aexp) : Int :=
   match a with
@@ -23,14 +32,22 @@ def store : Type := ident → Int
   | .PLUS a1 a2 => aeval s a1 + aeval s a2
   | .MINUS a1 a2 => aeval s a1 - aeval s a2
 
+/-
+Such evaluation functions / denotational semantics have many uses. First, we can use [aeval] to evaluate a given expression in a given store.
+-/
 /-- info: 3 -/
 #guard_msgs in
 #eval aeval (λ _ => 2) (.PLUS (.VAR "x") (.MINUS (.VAR "x") (.CONST 1)))
 
+-- We can prove properties of a given expression.
 theorem aeval_xplus1 : ∀ s x, aeval s (.PLUS (.VAR x) (.CONST 1)) > aeval s (.VAR x) := by
   grind
 
+/-
+  Finally, we can prove "meta-properties" that hold for all expressions. For example: the value of an expression depends only on the values of its free variables.
 
+  Free variables are defined by this recursive predicate:
+-/
 @[grind] def free_in_aexp (x : ident) (a : aexp) : Prop :=
   match a with
   | .CONST _ => False
@@ -44,14 +61,20 @@ theorem aeval_free :
     intro s1 _ a _
     fun_induction aeval s1 a with grind
 
-inductive bexp : Type where
-  | TRUE
-  | FALSE
-  | EQUAL (a1 : aexp) (a2 : aexp)
-  | LESSEQUAL (a1 : aexp) (a2 : aexp)
-  | NOT (b1 : bexp)
-  | AND (b1 : bexp) (b2 : bexp)
+/-
+  1.3 Boolean expressions
 
+  The IMP language has conditional statements (if/then/else) and loops.  They are controlled by expressions that evaluate to Boolean values.  Here is the abstract syntax of Boolean expressions.
+-/
+inductive bexp : Type where
+  | TRUE                            -- always true
+  | FALSE                           -- always false
+  | EQUAL (a1: aexp) (a2: aexp)     -- whether [a1=a]
+  | LESSEQUAL (a1: aexp) (a2: aexp) -- whether [a1≤a]
+  | NOT (b1: bexp)                  -- Boolean negation
+  | AND (b1: bexp) (b2: bexp)       -- Boolean conjunction
+
+-- There are many useful derived forms.
 def NOTEQUAL (a1 a2 : aexp) : bexp := .NOT (.EQUAL a1 a2)
 
 def GREATEREQUAL (a1 a2 : aexp) : bexp := .LESSEQUAL a2 a1
@@ -62,6 +85,9 @@ def LESS (a1 a2 : aexp) : bexp := GREATER a2 a1
 
 @[grind] def OR (b1 b2 : bexp) : bexp := .NOT (.AND (.NOT b1) (.NOT b2))
 
+/-
+Just like arithmetic expressions evaluate to integers, Boolean expressions evaluate to Boolean values `true` or `false`.
+-/
 @[grind] def beval (s : store) (b : bexp) : Bool :=
   match b with
   | .TRUE => true
@@ -71,18 +97,36 @@ def LESS (a1 a2 : aexp) : bexp := GREATER a2 a1
   | .NOT b1 =>  !(beval s b1)
   | .AND b1 b2 => beval s b1 && beval s b2
 
+-- We show the expected semantics for the `OR` derived form:
 theorem beval_OR :
   ∀ s b1 b2, beval s (OR b1 b2) = beval s b1 ∨ beval s b2 := by grind
 
-inductive com : Type where
-  | SKIP
-  | ASSIGN (x : ident) (a : aexp)
-  | SEQ (c1 : com) (c2 : com)
-  | IFTHENELSE (b : bexp) (c1 : com) (c2 : com)
-  | WHILE (b : bexp) (c1 : com)
+/-
+  1.4 Commands
 
+  To complete the definition of the IMP language, here is the abstract syntax of commands, also known as statements.
+-/
+inductive com: Type where
+  | SKIP                                      -- do nothing
+  | ASSIGN (x : ident) (a: aexp)              -- assignment: [v := a]
+  | SEQ (c1: com) (c2: com)                   -- sequence: [c1; c2]
+  | IFTHENELSE (b: bexp) (c1: com) (c2: com)  -- conditional: [if b then c1 else c2]
+  | WHILE (b: bexp) (c1: com)                 -- loop: [while b do c1 done]
+
+--  We can write `c1 ;; c2` instead of `.SEQ c1 c2`, it is easier on the eyes.
 notation:10 l:10 " ;; " r:11 => com.SEQ l r
 
+/-
+  Here is an IMP program that performs Euclidean division by
+  repeated subtraction.  At the end of the program, "q" contains
+  the quotient of "a" by "b", and "r" contains the remainder.
+  In pseudocode:
+  <<
+       r := a; q := 0;
+       while b <= r do r := r - b; q := q + 1 done
+  >>
+  In abstract syntax:
+-/
 def Euclidean_division :=
   .ASSIGN "r" (.VAR "a") ;;
   .ASSIGN "q" (.CONST 0) ;;
@@ -90,9 +134,43 @@ def Euclidean_division :=
     (.ASSIGN "r" (.MINUS (.VAR "r") (.VAR "b")) ;;
      .ASSIGN "q" (.PLUS (.VAR "q") (.CONST 1)))
 
+/-
+  A useful operation over stores:
+  `update x v s` is the store that maps `x` to `v` and is equal to `s` for all variables other than `x`.
+-/
 @[grind] def update (x : ident) (v : Int) (s : store) : store :=
   fun y => if x == y then v else s y
 
+/-
+  A naive approach to giving semantics to commands is to write an
+  evaluation function `cexec s c` that runs the command `c` in initial
+  store `s` and returns the final store when `c` terminates.
+
+  def cexec_fail (s: store) (c: com) : store :=
+    match c with
+    | .SKIP => s
+    | .ASSIGN x a => update x (aeval s a) s
+    | .SEQ c1 c2 => cexec_fail (cexec_fail s c1) c2
+    | .IFTHENELSE b c1 c2 => if beval s b then cexec_fail s c1 else cexec_fail s c2
+    | .WHILE b c1 =>
+        if beval s b
+        then (cexec_fail (cexec_fail s c1) (.WHILE b c1))
+        else s
+
+  The definition above is rejected by Lean, and rightly so, because
+  all Lean functions must terminate, yet the `.WHILE` case may not
+  terminate.  Consider for example the infinite loop `.WHILE .TRUE .SKIP`.
+
+  Worse, IMP is Turing-complete, since it has unbounded iteration
+  (`.WHILE`) plus arbitrary-precision integers.  Hence, there is no
+  computable function `cexec s c` that would return `.Some s'` if `c`
+  terminates with store `s'`, and `.none` if `c` does not terminate.
+
+  However, instead of computable functions, we can use a relation
+  `cexec s c s'` that holds iff command `c`, started in state `s`,
+  terminates with state `s'`.  This relation can easily be defined as
+  a Lean inductive predicate:
+-/
 @[grind] inductive cexec : store → com → store → Prop where
   | cexec_skip :
       cexec s .SKIP s
@@ -111,6 +189,11 @@ def Euclidean_division :=
       beval s b = true -> cexec s c s' -> cexec s' (.WHILE b c) s'' ->
       cexec s (.WHILE b c) s''
 
+/-
+  This style of semantics is known as natural semantics or big-step operational semantics.  The predicate `cexec s c s'` holds iff there exists a finite derivation of this conclusion, using the axioms and inference rules above.  The structure of the derivation represents the computations performed by `c` in a tree-like manner.  The finiteness of the derivation guarantees that only terminating executions satisfy `cexec`.
+
+  Indeed, `.WHILE .TRUE .SKIP` does not satisfy `cexec`:
+-/
 theorem cexec_infinite_loop :
   ∀ s, ¬ ∃ s', cexec s (.WHILE .TRUE .SKIP) s' := by
   intro _ h
@@ -120,6 +203,11 @@ theorem cexec_infinite_loop :
   intro h₂
   induction h₂ <;> grind
 
+/-
+  Our naive idea of an execution function for commands was not completely off.
+
+  We can define an approximation of such a function by bounding a priori the recursion depth, using a `fuel` parameter of type `Nat`.  When the fuel drops to `0`, `.none` is returned, meaning that the final store could not be computed.
+-/
 @[grind] def cexec_bounded (fuel : Nat) (s : store) (c : com) : Option store :=
   match fuel with
   | .zero => .none
@@ -141,6 +229,7 @@ theorem cexec_infinite_loop :
       else
         .some s
 
+--  We relate the `cexec` relation with the `cexec_bounded` function by proving the following two lemmas.
 theorem cexec_bounded_sound : ∀ fuel s c s',
     cexec_bounded fuel s c = .some s'
   → cexec s c s' := by
@@ -246,6 +335,17 @@ theorem cexec_bounded_complete (s s' : store) (c : com) :
         unfold cexec_bounded
         grind
 
+/-
+  6. Small-step semantics for IMP
+    6.1 Reduction semantics
+
+  In small-step style, the semantics is presented as a one-step
+  reduction relation ` red (c, s) (c', s') `, meaning that the command
+  `c`, executed in initial state `s`, performs one elementary step of
+  computation.  `s'` is the updated state after this step.  `c'` is
+  the residual command, capturing all the computations that remain to
+  be done.
+-/
 @[grind] inductive red : com × store → com × store → Prop where
   | red_assign : ∀ x a s,
       red (.ASSIGN x a, s) (.SKIP, update x (aeval s a) s)
@@ -263,6 +363,9 @@ theorem cexec_bounded_complete (s s' : store) (c : com) :
       beval s b = true →
       red (.WHILE b c, s) (.SEQ c (.WHILE b c), s)
 
+/-
+  We prove the following "progress" result for non-`SKIP` commands.
+-/
 theorem red_progress :
   ∀ c s, c = .SKIP ∨ ∃ c', ∃ s', red (c, s) (c', s') := by
     intro c
@@ -338,6 +441,7 @@ theorem red_progress :
 
 def goes_wrong (c : com) (s : store) : Prop := ∃ c', ∃ s', star red (c, s) (c', s') ∧ irred red (c', s') ∧ c' ≠ .SKIP
 
+-- Sequences of reductions can go under a sequence context, generalizing rule `.red_seq_step`.
 @[grind] theorem red_seq_steps (c2 c c' : com) (s s' : store) : star red (c, s) (c', s') → star red ((c;;c2), s) ((c';;c2), s') := by
   intro H
   generalize h₁ : (c,s) = v₁
@@ -358,6 +462,14 @@ def goes_wrong (c : com) (s : store) : Prop := ∃ c', ∃ s', star red (c, s) (
       · rfl
       · exact h₂
 
+/-
+  We now recall the equivalence result between
+  - termination according to the big-step semantics
+  - existence of a finite sequence of reductions to `SKIP`
+    according to the small-step semantics.
+
+  We start with the implication big-step ==> small-step, which is a straightforward induction on the big-step evaluation derivation.
+-/
 theorem cexec_to_reds (s s' : store) (c : com) : cexec s c s' → star red (c, s) (.SKIP, s') := by
   intro h
   induction h
@@ -382,6 +494,9 @@ theorem cexec_to_reds (s s' : store) (c : com) : cexec s c s' → star red (c, s
         · apply ih2
         · grind
 
+/-
+  The reverse implication, from small-step to big-step, is more subtle. The key lemma is the following, showing that one step of reduction followed by a big-step evaluation to a final state can be collapsed into a single big-step evaluation to that final state.
+-/
 @[grind] theorem red_append_cexec (c1 c2 : com) (s1 s2 : store) :
   red (c1, s1) (c2, s2) →
   ∀ s', cexec s2 c2 s' → cexec s1 c1 s' := by
@@ -400,6 +515,9 @@ theorem cexec_to_reds (s s' : store) (c : com) : cexec s c s' → star red (c, s
       · exact h2
     all_goals grind
 
+/-
+  As a consequence, a term that reduces to `SKIP` evaluates in big-step with the same final state.
+-/
 theorem reds_to_cexec (s s' : store) (c : com) :
   star red (c, s) (.SKIP, s') → cexec s c s' := by
     intro h
@@ -416,31 +534,67 @@ theorem reds_to_cexec (s s' : store) (c : com) :
       · apply a_ih
         all_goals grind
 
+/-
+  6.2 Transition semantics with continuations
+
+  We now introduce an alternate form of small-step semantics where the command to be executed is explicitly decomposed into:
+  - a sub-command under focus, where computation takes place;
+  - a continuation (or context) describing the position of this sub-command
+  in the whole command, or, equivalently, describing the parts of the
+  whole command that remain to be reduced once the sub-command is done.
+
+  As a consequence, the small-step semantics is presented as a transition relation between triples (subcommand-under-focus, continuation, state).  Previously, we had transitions between pairs (whole-command, state).
+
+  The syntax of continuations is as follows:
+-/
 @[grind] inductive cont where
 | Kstop
 | Kseq (c : com) (k : cont)
 | Kwhile (b : bexp) (c : com) (k : cont)
 
+/-
+  Intuitive meaning of these constructors:
+  - `.Kstop` means that, after the sub-command under focus terminates, nothing remains to be done, and execution can stop.  In other words, the sub-command under focus is the whole command.
+  - `.Kseq c k` means that, after the sub-command terminates, we still need to execute command `c` in sequence, then continue as described by `k`.
+- `.Kwhile b c k` means that, after the sub-command terminates, we still need to execute a loop [WHILE b DO c END], then continue as described by `k`.
+
+  Another way to forge intuitions about continuations is to ponder the following `apply_cont k c` function, which takes a sub-command `c` under focus and a continuation `k`, and rebuilds the whole command.  It simply puts `c` in lefmost position in a nest of sequences as described by `k`.
+-/
 @[grind] def apply_cont (k : cont) (c : com) : com :=
   match k with
   | .Kstop => c
   | .Kseq c1 k1 => apply_cont k1 (.SEQ c c1)
   | .Kwhile b1 c1 k1 => apply_cont k1 (.SEQ c (.WHILE b1 c1))
 
-inductive step : com × cont × store -> com × cont × store -> Prop where
-  | step_assign : ∀ x a k s,
+/-
+  Transitions between (subcommand-under-focus, continuation, state) triples perform conceptually different kinds of actions:
+  - Computation: evaluate an arithmetic expression or boolean expression and modify the triple according to the result of the evaluation.
+  - Focusing: replace the sub-command by a sub-sub-command that is to be evaluated next, possibly enriching the continuation as a consequence.
+  - Resumption: when the sub-command is `.SKIP` and therefore fully executed, look at the head of the continuation to see what to do next.
+
+  Here are the transition rules, classified by the kinds of actions they implement.
+-/
+inductive step: com × cont × store -> com × cont × store -> Prop where
+  | step_assign: forall x a k s,
       step (.ASSIGN x a, k, s) (.SKIP, k, update x (aeval s a) s)
-  | step_seq : ∀ c1 c2 s k,
+      -- computation for assignments
+  | step_seq: forall c1 c2 s k,
       step (.SEQ c1 c2, k, s) (c1, .Kseq c2 k, s)
-  | step_ifthenelse : ∀ b c1 c2 k s,
+      -- focusing for sequence
+  | step_ifthenelse: forall b c1 c2 k s,
       step (.IFTHENELSE b c1 c2, k, s) ((if beval s b then c1 else c2), k, s)
-  | step_while_done : ∀ b c k s,
+      -- computation for conditionals
+  | step_while_done: forall b c k s,
       beval s b = false ->
       step (.WHILE b c, k, s) (.SKIP, k, s)
-  | step_while_true : ∀ b c k s,
+      -- computation for loops
+  | step_while_true: forall b c k s,
       beval s b = true ->
       step (.WHILE b c, k, s) (c, .Kwhile b c k, s)
-  | step_skip_seq : ∀ c k s,
+      -- omputation and focusing for loops
+  | step_skip_seq: forall c k s,
       step (.SKIP, .Kseq c k, s) (c, k, s)
-  | step_skip_while : ∀ b c k s,
+      -- resumption
+  | step_skip_while: forall b c k s,
       step (.SKIP, .Kwhile b c k, s) (.WHILE b c, k, s)
+      -- resumption
